theories/L6_PCPS/L6_compose.v
@@ -1,0 +1,193 @@
+Require Import cps ctx cps_util List_util eval identifiers functions hoare Ensembles_util
+        closure_conversion closure_conversion_correct closure_conversion_corresp
+        hoisting logical_relations.
+(* Require Import Coq.ZArith.Znumtheory Coq.Relations.Relations Coq.Arith.Wf_nat. *)
+Require Import Coq.Lists.List Coq.MSets.MSets Coq.MSets.MSetRBT Coq.Numbers.BinNums
+        Coq.NArith.BinNat Coq.PArith.BinPos Coq.Sets.Ensembles Omega.
+Require Import ExtLib.Structures.Monads ExtLib.Data.Monads.StateMonad.
+
+
+Import ListNotations.
+
+Open Scope ctx_scope.
+Open Scope fun_scope.
+
+(** * Composition of L6 transformations and their correctness proofs *)
+
+
+Section L6_trans.
+   
+    Variable (clo_tag : cTag).
+    Variable (pr : prims).
+    Variable (cenv : cEnv).
+        
+    (** Top level correctness property of closure conversion and hoisting for closed terms *)
+    Corollary closure_conversion_hoist_correct k e ctag itag :
+      (* [e] is closed *)
+      closed_exp e ->
+      (* [e] has unique bindings *)
+      unique_bindings e ->
+      (* Then [e] and its translation are related by the logical relation *)
+      cc_approx_exp pr cenv clo_tag k
+                    (e, M.empty val)
+                    (closure_conversion_hoist clo_tag e ctag itag cenv, M.empty val).
+    Proof with now eauto with Ensembles_DB.
+      intros Hclo Hun.
+      unfold closure_conversion_hoist. 
+      set (S := fun y => BinPos.Pos.le (max_var e 1 + 1 + 1)%positive y).
+      set (s := {| next_var := (max_var e 1 + 1 + 1)%positive;
+                   nect_cTag := ctag;
+                   next_iTag := itag;
+                   closure_conversion.cenv := cenv |} ).
+      assert ({{ fun s : state_contents => fresh S (next_var s)}}
+                exp_closure_conv clo_tag e (Maps.PTree.empty VarInfo)
+                                 1%positive (max_var e 1 + 1)%positive
+              {{fun (_ : state_contents) (ef : exp * (exp -> exp))
+                  (_ : state_contents) =>
+                  let
+                    '(e', f) := ef in
+                  cc_approx_exp pr cenv clo_tag k (e, M.empty val) (f e', M.empty val) /\
+                  closed_exp (f e') /\
+                  unique_bindings (f e') /\
+                  closed_fundefs_in_exp (f e')
+               }}).
+      { eapply post_weakening;
+        [| eapply exp_closure_conv_correct_inv; try eassumption ].
+        - intros s1 [e' f] s2 _ [H1 [H2 [H3 [H4 _]]]]. split. eassumption.
+          split; [| now eauto ]. unfold closed_exp in *. rewrite Hclo in H2.
+          now split; eauto with Ensembles_DB.
+        - now apply FVmap_inv_empty.
+        - intros Hc. inv Hc.
+          eapply bound_var_leq_max_var with (y := 1%positive) in H.
+          zify; omega.
+          eapply occurs_free_leq_max_var with (y := 1%positive) in H.
+          zify; omega.
+        - unfold closed_exp in Hclo. intros x Hx. rewrite Hclo in Hx. inv Hx.
+        - unfold closed_exp in Hclo. intros x Hx. rewrite Hclo in Hx. inv Hx.
+        - intros x Hx. now apply M.gempty.
+        - intros x Hin. inv Hin.
+        - apply Union_Disjoint_r.
+          constructor. intros x Hc. 
+          inv Hc. eapply bound_var_leq_max_var with (y := 1%positive) in H0.
+          unfold S, In in H. zify; omega.
+          constructor. intros x Hc. 
+          inv Hc. inv H0. eapply occurs_free_leq_max_var with (y := 1%positive) in H1.
+          unfold S, In in H. zify; omega.
+          inv H1. unfold S, In in H. zify; omega. }
+      assert (Hf : fresh S (next_var s)) by (unfold S, s; intros x Hin; eauto).
+      unfold triple in H. specialize (H s Hf). 
+      destruct (runState _ _) as [[e' f] s'] eqn:Heq.
+      destruct H as [Hcc [Hclo' [Hun' HcloB]]].
+      eapply cc_approx_exp_respects_preord_exp_r with (e2 := f e').
+      eassumption.
+      intros k'. eapply hoist_exp_correct.
+      - eassumption.
+      - eassumption.
+      - unfold closed_exp in Hclo'. rewrite Hclo'...
+      - apply preord_env_P_refl.
+    Qed.
+    
+    (** Top level correctness property of closure conversion and hoisting for open terms *)
+    Corollary closure_conversion_hoist_open_correct k rho rho' e ctag itag :
+      (* [e] has unique bindings *)
+      unique_bindings e ->
+      (* the free variables of [e] are disjoint from the bound variables of [e] *)
+      Disjoint _ (bound_var e) (occurs_free e) ->
+      (* [rho] contains all the free variables of [e] *)
+      binding_in_map (occurs_free e) rho ->
+      (* [rho] and [rho'] are related by the closure conversion log. relation *)
+      cc_approx_env pr cenv clo_tag k rho rho' ->
+      (* Then [e] and its translation are related by the closure conversion log. relation *)
+      cc_approx_exp pr cenv clo_tag k
+                    (e, rho)
+                    (closure_conversion_hoist_open clo_tag rho e ctag itag cenv, rho').
+    Proof with now eauto with Ensembles_DB.
+      intros Hun HD Hbin Hcc.
+      unfold closure_conversion_hoist_open.
+      set (Γ := ((max_list (map fst (M.elements rho)) (max_var e 1)) + 1)%positive).
+      set (S := fun y => BinPos.Pos.le (Γ + 1)%positive y).
+      set (s := {| next_var := (Γ + 1)%positive;
+                   nect_cTag := ctag;
+                   next_iTag := itag;
+                   closure_conversion.cenv := cenv |} ).
+      set (map := fold_left
+                    (fun (map : M.t VarInfo) (p : M.elt * val) =>
+                       M.set (fst p) BoundVar map) (M.elements rho)
+                    (Maps.PTree.empty VarInfo)).
+      assert ({{ fun s : state_contents => fresh S (next_var s) }}
+                exp_closure_conv clo_tag e map 1%positive Γ
+                {{fun (_ : state_contents) (ef : exp * (exp -> exp))
+                    (_ : state_contents) =>
+                    let
+                      '(e', f) := ef in
+                    cc_approx_exp pr cenv clo_tag k (e, rho) (f e', rho') /\
+                    Included _ (occurs_free (f e')) (occurs_free e) /\
+                    unique_bindings (f e') /\
+                    closed_fundefs_in_exp (f e') /\
+                    Included _ (bound_var (f e'))
+                             (Union _ (bound_var e) S)
+                 }}).
+      { eapply post_weakening;
+        [| eapply exp_closure_conv_correct_inv
+           with (Scope := FromList (List.map fst (M.elements rho)));
+           try eassumption ].
+        - intros s1 [e' f] s2 _ [H1 [H2 [H3 [H4 H5]]]]. eauto.
+        - rewrite <- (Union_Empty_set_neut_r (FromList (List.map fst (M.elements rho))) ).
+          eapply populate_map_FVmap_inv. now apply FVmap_inv_empty.
+        - intros Hc. inv Hc.
+          eapply bound_var_leq_max_var with (y := 1%positive) in H.
+          eapply Pos.le_trans
+          with (p := max_list (List.map fst (M.elements rho)) (max_var e 1)) in H.
+          unfold Γ in H. zify; omega.
+          now apply max_list_spec1.
+          eapply binding_in_map_Included in H; [| eassumption ].
+          eapply max_list_spec2 with (z := (max_var e 1)) in H.
+          unfold Γ in H. zify; omega.
+        - eapply binding_in_map_antimon;
+          [| now eapply populate_map_binding_in_map with (S := Empty_set _);
+             intros x Hc; inv Hc ].
+          rewrite Union_Empty_set_neut_r. apply binding_in_map_Included.
+          eassumption.
+        - eapply populate_map_binding_not_in_map.
+          intros x Hc. now apply Maps.PTree.gempty. 
+          eapply Union_Disjoint_l.
+          constructor. intros x Hc. inv Hc.
+          unfold S, Γ, In in H. eapply max_list_spec2 with (z := max_var e 1) in H0.
+          zify; omega.
+          eapply Disjoint_Singleton_l. intros Hc.
+          eapply max_list_spec2 with (z := max_var e 1) in Hc.
+          unfold S, Γ in Hc. zify; omega.
+        - eapply cc_approx_env_P_antimon. eassumption.
+          now eauto with Ensembles_DB.
+        - apply Union_Disjoint_r.
+          constructor. intros x Hc. 
+          inv Hc. eapply bound_var_leq_max_var with (y := 1%positive) in H0.
+          eapply Pos.le_trans
+          with (p := max_list (List.map fst (M.elements rho)) (max_var e 1)) in H.
+          unfold S, In, Γ in H. zify; omega.
+          eapply Pos.le_trans. eassumption. now apply max_list_spec1.
+          apply Union_Disjoint_r.
+          constructor. intros x Hc. inv Hc.
+          eapply binding_in_map_Included in H0; [| eassumption ].
+          eapply max_list_spec2 with (z := (max_var e 1)) in H0.
+          unfold S, Γ, In in H. zify; omega.
+          eapply Disjoint_Singleton_r. intros Hc. 
+          unfold S, Γ, In in Hc. zify; omega. }
+      assert (Hf : fresh S (next_var s)) by (unfold S, s; intros x Hin; eauto).
+      unfold triple in H. specialize (H s Hf). 
+      destruct (runState _ _) as [[e' f] s'] eqn:Heq.
+      destruct H as [Hcc' [Hin1 [Hun' [HcloB Hin2]]]].
+      eapply cc_approx_exp_respects_preord_exp_r with (e2 := f e').
+      eassumption.
+      intros k'. eapply hoist_exp_correct; [ eassumption | eassumption | | ].
+      - eapply Disjoint_Included_r. eassumption.
+        eapply Disjoint_Included_l. eassumption.
+        eapply Union_Disjoint_l. eassumption.
+        constructor. intros x Hc. inv Hc.
+        eapply binding_in_map_Included in H0; [| eassumption ].
+        eapply max_list_spec2 with (z := (max_var e 1)) in H0.
+        unfold S, Γ, In in H. zify; omega.
+      - apply preord_env_P_refl.
+    Qed.  
+
+End L6_trans.
